having trouble with the toy example

verif/GlobalExtendsToy.v
@@ -1,7 +1,7 @@
 
 Require Import Coqlib.
 Require Import String.
-
+Require Import Lib.
 Definition ident : Type := Z * string.
 
 Definition ident_eq :
@@ -21,6 +21,41 @@ Inductive Expr :=
 | EList (l : list Expr)
 .
 
+Definition Expr_ind_full
+           (P : Expr -> Prop)
+           (Pl : list Expr -> Prop)
+           (PVar : forall id, P (EVar id))
+           (PConst : forall z, P (EConst z))
+           (PList : forall l, Pl l -> P (EList l))
+           (Hnil : Pl nil)
+           (Hcons : forall f r, P f -> Pl r -> Pl (f :: r))
+           (e : Expr)
+  : P e :=
+  let fix go e :=
+  let fix go_list l :=
+      match l as _l return Pl _l with
+      | nil => Hnil
+      | f :: r => Hcons f r (go f) (go_list r)
+      end in
+  match e with
+  | EVar id => PVar id
+  | EConst z => PConst z
+  | EList l => PList l (go_list l)
+  end in
+  go e.
+
+Definition Expr_ind_useful
+           (P : Expr -> Prop)
+           (PVar : forall id, P (EVar id))
+           (PConst : forall z, P (EConst z))
+           (PList : forall l, Forall P l -> P (EList l))
+           (e : Expr)
+  : P e.
+  eapply Expr_ind_full. eauto. eauto.
+  eapply PList. econstructor.
+  intros. econstructor; eauto.
+Defined.
+
 Inductive val :=
 | num (z : Z)
 | listval (l : list val)
@@ -30,25 +65,107 @@ Definition genv : Type := ident -> option Expr.
 Definition gempty : genv := fun _ => None.
 Definition env : Type := ident -> option val.
 
-Inductive eval_expr (ge : genv) : env -> Expr -> val -> Prop :=
+Inductive eval_expr : genv -> env -> Expr -> val -> Prop :=
 | eval_global_var :
-    forall id E v e,
+    forall ge id E v e,
       ge id = Some e ->
       E id = None ->
       eval_expr ge E e v -> (* This line is the killer *)
       eval_expr ge E (EVar id) v
 | eval_list :
-    forall l vs E,
+    forall ge l vs E,
       Forall2 (eval_expr ge E) l vs ->
       eval_expr ge E (EList l) (listval vs)
 | eval_local_var :
-    forall id E v,
+    forall ge id E v,
       E id = Some v ->
       eval_expr ge E (EVar id) v
 | eval_const :
-    forall z E,
+    forall ge z E,
       eval_expr ge E (EConst z) (num z)
 .
+
+
+Definition widens (ge : genv) (e : Expr) : Prop :=
+  forall E v,
+    eval_expr ge E e v ->
+    forall id exp,
+      ge id = None ->
+      eval_expr (extend ge id exp) E e v.
+
+
+Lemma widens_ge :
+  forall e (ge : genv),
+    (forall id e, ge id = Some e -> widens ge e) ->
+    widens ge e.
+Proof.
+  induction e; intros.
+  unfold widens. intros. inversion H0. subst. econstructor; eauto.
+  unfold extend. destruct (ident_eq id id0). admit.
+  eassumption.
+  eapply H in H3. eapply H3. eauto. eauto.
+  eapply eval_local_var. eauto.
+  unfold widens. intros.
+  inversion H0.
+  econstructor; eauto.
+  unfold widens.
+  intros.
+  inversion H0. subst.
+  econstructor.
+  eapply Forall_Forall2_implies; try eassumption.
+Admitted. (* we can prove this *)  
+  
+Lemma ge_widens_empty :
+  forall ge e,
+    (forall id, ge id = None) ->
+    widens ge e.
+Proof.
+  unfold widens.
+  intros.
+  eapply widens_ge; eauto.
+  intros.
+  rewrite H in H2. congruence.
+Qed.
+
+Lemma widens_out :
+  forall (ge : genv),
+    (forall id e, ge id = Some e -> widens ge e) ->
+    forall idNew eNew,
+      forall id e, (extend ge idNew eNew) id = Some e -> widens (extend ge idNew eNew) e.
+Proof.
+  (* If we can prove this, we're set? *)
+Admitted.
+
+Fixpoint make_ge (l : list (ident * Expr)) (ge : genv) : genv :=
+  match l with
+  | nil => ge
+  | (id,exp) :: l' =>
+    let ge' := make_ge l' ge in
+    extend ge' id exp
+  end.
+
+
+Definition finite' (ge : genv) (l : list (ident * Expr)) : Prop :=
+  forall id,
+    ge id = make_ge l gempty id.
+
+Lemma all_widens :
+  forall l ge,
+    finite' ge l ->
+    forall e,
+      widens ge e.
+Proof.
+  induction l; intros.
+  unfold finite' in *.
+  eapply ge_widens_empty.
+  intros. rewrite H. simpl. unfold gempty. reflexivity.
+
+  (* How do I prove this? *)
+Admitted.
+
+(* we can prove that any expression widens, given that everything in the environment widens *)
+(* what is hard is proving that everything in the environment widens *)
+
 
 Fixpoint lookup (id : ident) (l : list (ident * Expr)) : option Expr :=
   match l with
@@ -77,6 +194,14 @@ Inductive eval_expr_listenv : list (ident * Expr) -> env -> Expr -> val -> Prop 
       eval_expr_listenv ge E (EConst z) (num z)
 .
 
+
+(* There isn't a counterexample here *)
+(* rather the problem is that the Inductive hypothesis is not strong enough *)
+
+(* We need to be able to simultaneously add something to the global
+environment, while showing that all previous expressions still
+evaluate to the same thing under this new global environment *)
+
 (*
 Lemma eval_expr_listenv_swap :
   forall ge E expr v,
@@ -90,17 +215,7 @@ Proof.
  *)
 
 (*
-Fixpoint make_ge (l : list (ident * Expr)) (ge : genv) : genv :=
-  match l with
-  | nil => ge
-  | (id,exp) :: l' =>
-    let ge' := make_ge l' ge in
-    extend ge' id exp
-  end.
 
-Definition finite' (ge : genv) (l : list (ident * Expr)) : Prop :=
-  forall id,
-    ge id = make_ge l gempty id.
 *)
 
 Lemma eval_expr_swap_ge :
